class

src/part1/Relations.lean
@@ -2,6 +2,18 @@ open Nat
 
 namespace Relations
 
+inductive True : Prop where
+| tt : True
+
+inductive False : Prop where
+-- this line deliberately left blank
+
+theorem ex_quod_libet : ∀ (P : Prop), False → P
+  := by
+       intros P f
+       cases f
+
+
 inductive le : Nat → Nat → Prop
 | refl : ∀ {m}, le m m
 | step : ∀ {m n}, le m n → le m (succ n)
@@ -16,27 +28,57 @@ def lt (n m : Nat) := le (succ n) m
 instance : LT Nat where
   lt := lt
 
-def invert : ∀ {m n : Nat}, succ m ≤ succ n -> m ≤ n
+theorem invert : ∀ {m n : Nat}, succ m ≤ succ n -> m ≤ n
   := by
-      intros m n m_le_n
-      cases m_le_n with
+      intros m n sm_le_sn
+      cases sm_le_sn with
       | refl =>
          exact refl
-      | step m_le_n =>
-        cases n with
-        | zero => contradiction
-        | succ n => apply step; apply invert; assumption
+      | step sm_le_n =>
+         cases n with
+         | zero => contradiction
+         | succ n => apply step; apply invert; assumption
 
 -- Proof is by induction, but induction tactic does not apply.
 -- Note explicit application of "invert"
 
-def trans_le : ∀ {m n p : Nat}, m ≤ n → n ≤ p → m ≤ p
+[@trans] def trans_le : ∀ {m n p : Nat}, m ≤ n → n ≤ p → m ≤ p
   := by
        intros m n p m_le_n n_le_p
        induction n_le_p with
        | refl => assumption
        | step n_le_p ih => apply step; exact ih
 
+example : 2 ≤ 5 :=
+  calc
+    2 ≤ 2  := refl
+    _ ≤ 3  := step _
+
+-- Exercise.
+-- Here is a different definition of ≤.
+-- Prove the two definitions equivalent,
+-- that is, that each implies the other.
+
+inductive le2 : Nat → Nat → Prop
+| z_le_n :
+      ----------
+      le2 zero n
+| s_le_s :
+      le2 m n
+      ---------------------
+    → le2 (succ m) (succ n)
+
+open le2
+
+-- Exercise.
+-- Prove lt and lt2 equivalent.
+
+inductive lt2 : Nat → Nat → Prop where
+| z_lt_s : ∀ {n}, lt2 zero (succ n)
+| s_lt_s : ∀ {m n},
+      lt2 m n
+      ---------------------
+    → lt2 (succ m) (succ n)
 
 
 
